

Ejercicio 2)

Utilizando orden normal obtenemos:

$((\lambda z.z \lambda t.(t z)) (\lambda w.\lambda x.(w x) (x x)))$

Reglas aplicadas Resultado

Regla β	=	$([\lambda t.(t z) / z] z (\lambda w.\lambda x.(w x) (x x)))$
1	=	$(\lambda t.(t z) (\lambda w.\lambda x.(w x) (x x)))$
Regla β	=	$[(\lambda w.\lambda x.(w x) (x x)) / t] (t z)$
3	=	$(([\lambda w.\lambda x.(w x) (x x)) / t] t [(\lambda w.\lambda x.(w x) (x x)) / t] z)$
1, 2	=	$((\lambda w.\lambda x.(w x) (x x)) z)$
Regla β	=	$([(x x) / w] \lambda x.(w x) z)$
6	=	$(\lambda y.[(x x) / w] [y / x] (w x) z)$
3	=	$(\lambda y.[(x x) / w] ([y / x] w [y / x] x) z)$
2, 1	=	$(\lambda y.[(x x) / w] (w y) z)$
3	=	$(\lambda y.([(x x) / w] w [(x x) / w] y) z)$
1, 2	=	$(\lambda y.((x x) y) z)$
Regla β	=	$[z / y] ((x x) y)$
3, 3	=	$(([z / y] x [z / y] x) [z / y] y)$
1, 1, 2	=	$((x x) z) \rightarrow \text{FORMA NORMAL}$

Ejercicio 2)

Utilizando orden normal obtenemos:

$(\lambda x.(x\ x)\ \lambda y.(\lambda x.(y\ x)\ \lambda y.y))$

Reglas aplicadas Resultado

Regla β	=	$[\lambda y.(\lambda x.(y\ x)\ \lambda y.y) / x] (x\ x)$
3	=	$([\lambda y.(\lambda x.(y\ x)\ \lambda y.y) / x] x\ [\lambda y.(\lambda x.(y\ x)\ \lambda y.y) / x] x)$
1, 1	=	$(\lambda y.(\lambda x.(y\ x)\ \lambda y.y)\ \lambda y.(\lambda x.(y\ x)\ \lambda y.y))$
Regla β	=	$[\lambda y.(\lambda x.(y\ x)\ \lambda y.y) / y] (\lambda x.(y\ x)\ \lambda y.y)$
3	=	$([\lambda y.(\lambda x.(y\ x)\ \lambda y.y) / y] \lambda x.(y\ x)\ [\lambda y.(\lambda x.(y\ x)\ \lambda y.y) / y] \lambda y.y)$
5, 4	=	$(\lambda x.[\lambda y.(\lambda x.(y\ x)\ \lambda y.y) / y] (y\ x)\ \lambda y.y)$
3	=	$(\lambda x.([\lambda y.(\lambda x.(y\ x)\ \lambda y.y) / y] y\ [\lambda y.(\lambda x.(y\ x)\ \lambda y.y) / y] x)\ \lambda y.y)$
1, 2	=	$(\lambda x.(\lambda y.(\lambda x.(y\ x)\ \lambda y.y)\ x)\ \lambda y.y)$
Regla β	=	$[\lambda y.y / x] (\lambda y.(\lambda x.(y\ x)\ \lambda y.y)\ x)$
3	=	$([\lambda y.y / x] \lambda y.(\lambda x.(y\ x)\ \lambda y.y)\ [\lambda y.y / x] x)$
5, 1	=	$(\lambda y.[\lambda y.y / x] (\lambda x.(y\ x)\ \lambda y.y)\ \lambda y.y)$
3	=	$(\lambda y.([\lambda y.y / x] \lambda x.(y\ x)\ [\lambda y.y / x] \lambda y.y)\ \lambda y.y)$
4	=	$(\lambda y.(\lambda x.(y\ x)\ [\lambda y.y / x] \lambda y.y)\ \lambda y.y)$
5	=	$(\lambda y.(\lambda x.(y\ x)\ \lambda y.[\lambda y.y / x] y)\ \lambda y.y)$
2	=	$(\lambda y.(\lambda x.(y\ x)\ \lambda y.y)\ \lambda y.y)$
Regla β	=	$[\lambda y.y / y] (\lambda x.(y\ x)\ \lambda y.y)$
3	=	$([\lambda y.y / y] \lambda x.(y\ x)\ [\lambda y.y / y] \lambda y.y)$
5, 4	=	$(\lambda x.[\lambda y.y / y] (y\ x)\ \lambda y.y)$
3	=	$(\lambda x.([\lambda y.y / y] y\ [\lambda y.y / y] x)\ \lambda y.y)$
1, 2	=	$(\lambda x.(\lambda y.y\ x)\ \lambda y.y)$
Regla β	=	$[\lambda y.y / x] (\lambda y.y\ x)$
3	=	$([\lambda y.y / x] \lambda y.y\ [\lambda y.y / x] x)$
5, 1	=	$(\lambda y.[\lambda y.y / x] y\ \lambda y.y)$
2	=	$(\lambda y.y\ \lambda y.y)$
Regla β	=	$[\lambda y.y / y] y$
1	=	$\lambda y.y \rightarrow \text{FORMA NORMAL}$